# HL_04_25_22

## 7.1 The Substitution Rule
#### Question 5
Evaluate this integral using u-substitution
```math
\int \frac{2x^4}{6-x^5}dx\\
```
Make a u-substitution then take the derivative 
```math
u=6-x^5\\
du = -5x^4dx\\
dx = -\frac{du}{5x^4}
```
Replace your $6-x^5$ and your $dx$
```math
\int \frac{2x^4}{u}(-\frac{du}{5x^4})\\
```
Notice that the $x^4$'s cancel out. The $-\frac{2}{5}$ is factored out.
```math
-\frac{2}{5}\int\frac{1}{u}du = -\frac{2}{5}ln|u|= -\frac{2}{5}ln|6-x^5| + C
```
Do not forget to add C when evaluating indefinite integrals.

#### Question 5
![clipboard.png](S6CuDogc3-clipboard.png)

Lets perform u-substitution. Let $u=x^5-5x^3+4$
```math
du =(5x^4-15x^2)dx\\
dx = \frac{du}{5x^4-15x^2}
```
Replace
```math
\int\frac{(x^4-3x^2)u^{1/5}}{5x^4-15x^2}du \\
```
Factor out the $5$ in the denominator and push to the front
```math
\frac{1}{5}\int\frac{(x^4-3x^2)u^{1/5}}{x^4-3x^2}du
```
Cancel out the factors of $x$
```math
\frac{1}{5}\int u^{1/5}du = \frac{1}{5}\frac{u^{6/5}}{6/5}=\frac{1}{5}\frac{5}{6}u^{6/5}=\frac{u^{6/5}}{6}=\frac{(x^5-5x^3+4)^{6/5}}{6}+C
```
#### Question 5
![clipboard.png](5Df9ZKLPQ-clipboard.png)

Let $u=sinx$
```math
du = cosxdx\\
dx = \frac{du}{cosx}
```
Replace
```math
\int u^7cos(x)(\frac{du}{cosx})
```
Notice the $cos(x)$ cancels out
```math
\int u^7du = \frac{sin(x)^8}{8}+C
```
#### Problem 10
![clipboard.png](DU7Jsvh9v-clipboard.png)

Let $u=ln(4x-1)$
```math
du=\frac{4}{4x-1}dx\\
dx = \frac{4x-1}{4}du
```
Replace and cancel out
```math
\int\frac{4}{4x-1}\frac{1}{u}\frac{4x-1}{4}du\\
= \int\frac{1}{u}du
= ln|ln(4x-1)|+C
```
#### Problem 13
![clipboard.png](06pKpvkO_-clipboard.png)

Let $u=e^x+1$
```math
dx = \frac{du}{e^x}\\
=\int_{ln5}^{ln9}\frac{e^x}{u^2}\frac{du}{e^x}\\
=\int_{ln5}^{ln9}u^{-2}du\\
=-\frac{1}{e^x+1}\bigg|_{ln5}^{ln9}\\
-(\frac{1}{10}-\frac{1}{6})